\documentclass[12pt, letterpaper]{extarticle}

\input{Configs}

\begin{document}

% \subfile{Portada.tex}

% \newpage

% \tableofcontents

% \newpage

\newSection{Embragues, frenos, coples y volantes de inercia}

\newSubSection{Embragues y frenos de tambor de expansión interna}

\begin{align*}
    M_{f} &= \frac{fp_{a}br}{\sin(\theta_{a})} \int_{\theta_{1}}^{\theta_{2}} \sin(\theta) (r - a\cos(\theta)) \; d\theta \\
    M_{n} &= \frac{p_{a}bra}{\sin(\theta_{a})} \int_{\theta_{1}}^{\theta_{2}} \sin^{2}(\theta) \; d\theta
\end{align*}

\begin{align*}
    A &= \int_{\theta_{1}}^{\theta_{2}} \sin(\theta)\cos(\theta) \; d\theta = \left.\left(\frac{1}{2}\sin^{2}(\theta)\right) \right|_{\theta_{1}}^{\theta_{2}} \\
    B &= \int_{\theta_{1}}^{\theta_{2}} \sin^{2}(\theta) \; d\theta = \left.\left(\frac{\theta}{2} - \frac{1}{4}\sin(2\theta)\right) \right|_{\theta_{1}}^{\theta_{2}}
\end{align*}

\begin{equation*}
    T = \frac{fp_{a}br^2(\cos(\theta_{1}) - \cos(\theta_{2}))}{\sin(\theta_{a})}
\end{equation*}


\newSubSubSection{Caso I (fuerza $\rightarrow$ pasador)}

\begin{equation*}
    F = \frac{M_{n} - M_{f}}{c}
\end{equation*}

\begin{align*}
    R_{x} &= \frac{p_{a}br}{\sin(\theta_{a})}(A - fB) - F_{x} \\
    R_{y} &= \frac{p_{a}br}{\sin(\theta_{a})}(B + fA) - F_{y}
\end{align*}

\newSubSubSection{Caso II (pasador $\rightarrow$ fuerza)}

\begin{equation*}
    F = \frac{M_{n} + M_{f}}{c}
\end{equation*}

\begin{align*}
    R_{x} &= \frac{p_{a}br}{\sin(\theta_{a})}(A + fB) - F_{x} \\
    R_{y} &= \frac{p_{a}br}{\sin(\theta_{a})}(B - fA) - F_{y}
\end{align*}

\newpage
\newSubSection{Embragues y frenos de contracción externa}

\begin{align*}
    M_{f} &= \frac{fp_{a}br}{\sin(\theta_{a})} \int_{\theta_{1}}^{\theta_{2}} \sin(\theta) (r - a\cos(\theta)) \; d\theta \\
    M_{n} &= \frac{p_{a}bra}{\sin(\theta_{a})} \int_{\theta_{1}}^{\theta_{2}} \sin^{2}(\theta) \; d\theta
\end{align*}

\begin{align*}
    A &= \int_{\theta_{1}}^{\theta_{2}} \sin(\theta)\cos(\theta) \; d\theta = \left.\left(\frac{1}{2}\sin^{2}(\theta)\right) \right|_{\theta_{1}}^{\theta_{2}} \\
    B &= \int_{\theta_{1}}^{\theta_{2}} \sin^{2}(\theta) \; d\theta = \left.\left(\frac{\theta}{2} - \frac{1}{4}\sin(2\theta)\right) \right|_{\theta_{1}}^{\theta_{2}}
\end{align*}

\begin{equation*}
    T = \frac{fp_{a}br^2(\cos(\theta_{1}) - \cos(\theta_{2}))}{\sin(\theta_{a})}
\end{equation*}

\newSubSubSection{Caso I (fuerza $\rightarrow$ pasador)}

\begin{equation*}
    F = \frac{M_{n} + M_{f}}{c}
\end{equation*}

\begin{align*}
    R_{x} &= \frac{p_{a}br}{\sin(\theta_{a})}(A + fB) - F_{x} \\
    R_{y} &= \frac{p_{a}br}{\sin(\theta_{a})}(fA - B) + F_{y}
\end{align*}

\newSubSubSection{Caso II (pasador $\rightarrow$ fuerza)}

\begin{equation*}
    F = \frac{M_{n} - M_{f}}{c}
\end{equation*}

\begin{align*}
    R_{x} &= \frac{p_{a}br}{\sin(\theta_{a})}(A - fB) - F_{x} \\
    R_{y} &= \frac{p_{a}br}{\sin(\theta_{a})}(-fA - B) + F_{y}
\end{align*}

\end{document}